PDDL_Instance_Relationships.thy
@@ -1,0 +1,63 @@
+theory PDDL_Instance_Relationships
+imports PDDL_Sema_Supplement
+begin
+
+text \<open>This theory concerns itself mostly with relationships between two PDDL instances
+  (domains or problems). They are of particular interest since the normalization steps produce
+  new instances that retain some of the previous properties.\<close>
+
+lemma co_fmla_wf:
+  assumes "\<And>a. ast_domain.wf_atom d1 tyt1 a \<longrightarrow> ast_domain.wf_atom d2 tyt2 a"
+  shows "ast_domain.wf_fmla d1 tyt1 \<phi> \<longrightarrow> ast_domain.wf_fmla d2 tyt2 \<phi>"
+  using assms apply (induction \<phi>)
+  using ast_domain.wf_fmla.simps apply metis+
+  done
+
+lemma co_fmla_atom_wf:
+  assumes "\<And>a. ast_domain.wf_atom d1 tyt1 a \<longrightarrow> ast_domain.wf_atom d2 tyt2 a"
+  shows "ast_domain.wf_fmla_atom d1 tyt1 \<phi> \<longrightarrow> ast_domain.wf_fmla_atom d2 tyt2 \<phi>"
+  using assms co_fmla_wf ast_domain.wf_fmla_atom_alt by metis
+
+lemma co_effect_wf:
+  assumes "\<And>a. ast_domain.wf_atom d1 tyt1 a \<longrightarrow> ast_domain.wf_atom d2 tyt2 a"
+  shows "ast_domain.wf_effect d1 tyt1 \<epsilon> \<longrightarrow> ast_domain.wf_effect d2 tyt2 \<epsilon>"
+  using assms co_fmla_atom_wf ast_domain.wf_effect_alt by metis
+
+lemma co_wm_wf:
+  assumes "\<And>a. ast_domain.wf_atom (domain p1) (ast_problem.objT p1) a
+    \<longrightarrow> ast_domain.wf_atom (domain p2) (ast_problem.objT p2) a"
+  shows "ast_problem.wf_world_model p1 m \<longrightarrow> ast_problem.wf_world_model p2 m"
+  using assms co_fmla_atom_wf ast_problem.wf_world_model_def by metis
+
+lemmas co_wf = co_fmla_wf co_fmla_atom_wf co_effect_wf co_wm_wf
+
+subsection \<open> Formula Preds \<close>
+
+fun fmla_preds :: "'ent atom formula \<Rightarrow> predicate set" where
+  "fmla_preds (Atom (predAtm p xs)) = {p}" |
+  "fmla_preds (Atom (Eq a b)) = {}" |
+  "fmla_preds \<bottom> = {}" |
+  "fmla_preds (\<^bold>\<not> \<phi>) = fmla_preds \<phi>" |
+  "fmla_preds (\<phi>\<^sub>1 \<^bold>\<and> \<phi>\<^sub>2) = fmla_preds \<phi>\<^sub>1 \<union> fmla_preds \<phi>\<^sub>2" |
+  "fmla_preds (\<phi>\<^sub>1 \<^bold>\<or> \<phi>\<^sub>2) = fmla_preds \<phi>\<^sub>1 \<union> fmla_preds \<phi>\<^sub>2" |
+  "fmla_preds (\<phi>\<^sub>1 \<^bold>\<rightarrow> \<phi>\<^sub>2) = fmla_preds \<phi>\<^sub>1 \<union> fmla_preds \<phi>\<^sub>2"
+
+lemma fmla_preds_alt: "fmla_preds \<phi> = {p | p xs. predAtm p xs \<in> atoms \<phi>}"
+  apply (induction \<phi>)
+  subgoal for x
+    apply (cases x; simp_all)
+    done
+  by auto
+
+
+lemma map_preserves_fmla_preds: "fmla_preds F = fmla_preds ((map_formula \<circ> map_atom) f F)"
+proof (induction F)
+  case (Atom x)
+  thus ?case by (cases x) simp_all
+qed auto
+
+lemma notin_fmla_preds_notin_atoms: "p \<notin> fmla_preds \<phi> \<Longrightarrow> predAtm p args \<notin> atoms \<phi>"
+  using fmla_preds_alt by blast
+
+
+end
