PDDL_Sema_Supplement.thy
@@ -1,0 +1,320 @@
+theory PDDL_Sema_Supplement
+  imports "AI_Planning_Languages_Semantics.PDDL_STRIPS_Semantics"
+  Utils
+begin
+
+(* not much here yet *)
+find_theorems name: "wf_ast_domain."
+find_theorems name: "wf_ast_problem."
+
+(* wf_domain unfolded and split *)
+lemmas (in wf_ast_domain) wf_D = conj_split_7[OF wf_domain[unfolded wf_domain_def]]
+
+(* wf_problem unfolded and split, but omitting the first fact "wf_domain" *)
+lemmas (in wf_ast_problem) wf_P =
+  conj_split_5[OF wf_problem[unfolded wf_problem_def, THEN conjunct2]]
+
+lemmas (in wf_ast_problem) wf_DP = wf_D wf_domain wf_P
+
+declare ast_problem.I_def[simp]
+
+subsection \<open> Accessor functions \<close>
+
+(* what's the builtin way? *)
+fun un_Atom :: "'a formula \<Rightarrow> 'a" where
+  "un_Atom (Atom x) = x" |
+  "un_Atom _ = undefined"
+
+abbreviation "unPredAtom \<equiv> predicate \<circ> un_Atom"
+
+abbreviation (input) get_t :: "type \<Rightarrow> name" where
+    "get_t T \<equiv> hd (primitives T)"
+lemma get_t_alt: "get_t (Either (t # ts)) = t"
+  by simp
+
+lemma is_predAtom_decomp: assumes "is_predAtom \<phi>"
+  obtains p xs where "\<phi> = Atom (predAtm p xs)"
+  using assms apply (cases \<phi>)
+  apply (meson is_predAtom.elims(2))
+  by simp_all
+
+abbreviation "ac_name \<equiv> ast_action_schema.name"
+abbreviation "ac_params \<equiv> ast_action_schema.parameters"
+abbreviation "ac_pre \<equiv> ast_action_schema.precondition"
+abbreviation "ac_eff \<equiv> ast_action_schema.effect"
+
+abbreviation (in ast_domain) pred_names :: "name list" where
+    "pred_names \<equiv> map (predicate.name \<circ> pred) (predicates D)"
+
+abbreviation (in ast_problem) "all_consts \<equiv> consts D @ objects P"
+
+subsection \<open>Alternative definitions\<close>
+
+text \<open>Alternative definitions. Most of these just remove pattern matching
+  from functions, e.g. a function "add (x, y) = x + y" would be turned into
+  "add p = fst p + snd p".
+  They are often unnecessary because you can just apply "cases" in a proof.
+  Others functions are only well-defined if a certain condition holds. The _cond-lemmas
+  help resolve it directly. \<close>
+
+abbreviation "map_atom_fmla \<equiv> map_formula \<circ> map_atom"
+
+context ast_domain begin
+(* unnecessary? *)
+lemma apply_effect_alt: "apply_effect \<epsilon> s = (s - set (dels \<epsilon>)) \<union> (set (adds \<epsilon>))"
+  by (cases \<epsilon>; simp_all)
+
+lemma subtype_edge_swap: "subtype_edge = prod.swap"
+  by (intro ext; auto)
+
+lemma subtype_rel_alt: "subtype_rel = (set (types D))\<inverse>"
+  unfolding subtype_rel_def
+  by (subst subtype_edge_swap; auto)
+
+lemma subtype_rel_star_alt: "subtype_rel\<^sup>* = ((set (types D))\<^sup>*)\<inverse>"
+    using subtype_rel_alt rtrancl_converse by simp
+
+(* useless? *)
+lemmas wf_atom_deep = wf_atom.simps[unfolded wf_pred_atom.simps]
+
+lemma wf_effect_alt:
+    "wf_effect tyt \<epsilon> \<longleftrightarrow>
+        (list_all1 (wf_fmla_atom tyt) (adds \<epsilon>))
+      \<and> (list_all1 (wf_fmla_atom tyt) (dels \<epsilon>))"
+  by (cases \<epsilon>; simp add: list_all_def)
+
+abbreviation "ac_tyt a \<equiv> ty_term (map_of (ac_params a)) constT"
+
+lemma wf_action_schema_alt: "wf_action_schema ac \<longleftrightarrow>
+    distinct (map fst (ac_params ac))
+  \<and> wf_fmla (ac_tyt ac) (ac_pre ac)
+  \<and> wf_effect (ac_tyt ac) (ac_eff ac)"
+  apply (cases ac; simp)
+  unfolding Let_def by simp
+
+(* unnecessary? *)
+lemma wf_type_alt: "wf_type T \<longleftrightarrow> set (primitives T) \<subseteq> insert ''object'' (fst ` set (types D))"
+  by (cases T; simp)
+
+(* unnecessary? *)
+lemma wf_predicate_decl_alt: "wf_predicate_decl pd \<longleftrightarrow> list_all1 wf_type (argTs pd)"
+  by (cases pd; simp)
+
+lemma (in wf_ast_domain) resolve_action_schema_cond:
+  assumes "Action_Schema n params pre eff \<in> set (actions D)"
+  shows "resolve_action_schema n = Some (Action_Schema n params pre eff)"
+  using assms wf_D(6)
+  by (simp add: resolve_action_schema_def)
+
+definition (in -) ac_tsubst :: "(variable \<times> type) list \<Rightarrow> object list \<Rightarrow> (PDDL_STRIPS_Semantics.term \<Rightarrow> object)" where
+  [simp]: "ac_tsubst params args \<equiv> ast_domain.subst_term (the \<circ> (map_of (zip (map fst params) args)))"
+
+lemma instantiate_action_schema_alt: "instantiate_action_schema ac args = Ground_Action
+  (map_atom_fmla (ac_tsubst (ac_params ac) args) (ac_pre ac))
+  (map_ast_effect (ac_tsubst (ac_params ac) args) (ac_eff ac))"
+  apply (cases ac; simp)
+  using ac_tsubst_def by metis
+
+end
+context ast_problem begin
+
+lemma resolve_instantiate_alt: "resolve_instantiate \<pi> =
+  instantiate_action_schema (the (resolve_action_schema (name \<pi>))) (arguments \<pi>)"
+  by (cases \<pi>; simp)
+
+lemma (in wf_ast_problem) resolve_instantiate_cond:
+  assumes "Action_Schema n params pre eff \<in> set (actions D)"
+  shows "resolve_instantiate (PAction n args) = Ground_Action
+    (map_atom_fmla (ac_tsubst params args) pre)
+    (map_ast_effect (ac_tsubst params args) eff)"
+  using assms apply (simp add: resolve_action_schema_cond del: instantiate_action_schema.simps)
+  by (simp add: instantiate_action_schema_alt)
+
+(* removing the redundant conjunct from the definition of wf_plan_action *)
+lemma (in wf_ast_problem) wf_plan_action_simple:
+  "wf_plan_action (PAction n args) \<longleftrightarrow> (case resolve_action_schema n of
+    None \<Rightarrow> False | Some a \<Rightarrow> action_params_match a args)"
+  apply (rule iffI)
+   apply (simp_all split: option.splits)
+  using wf_DP(7)
+  by (metis ground_action.collapse index_by_eq_SomeD wf_instantiate_action_schema resolve_action_schema_def wf_effect_inst_alt wf_ground_action.simps)
+
+(* unnecessary? *)
+lemma (in wf_ast_problem) wf_plan_action_alt: "wf_plan_action \<pi> \<longleftrightarrow>
+  (case resolve_action_schema (name \<pi>) of
+    None \<Rightarrow> False |
+    Some a \<Rightarrow> action_params_match a (arguments \<pi>))"
+  apply (cases \<pi>)
+  using wf_plan_action_simple plan_action.sel by presburger
+
+lemma (in wf_ast_problem) wf_plan_action_cond:
+  assumes "Action_Schema n params pre eff \<in> set (actions D)"
+  shows "wf_plan_action (PAction n args) \<longleftrightarrow>
+    action_params_match (Action_Schema n params pre eff) args"
+  using assms wf_plan_action_simple resolve_action_schema_cond
+  by (metis option.simps(5))
+
+(* unnecessary? *)
+lemma wf_ground_action_alt: "wf_ground_action ga \<longleftrightarrow>
+  wf_fmla objT (precondition ga) \<and> wf_effect objT (effect ga)"
+  by (cases ga; simp)
+
+text \<open> Note to self: ground_action_path checks if preconditions are enabled,
+but plan_action_path only checks it via ground_action_path.
+I don't see any redundancy. plan_action_enabled is only used in proofs. \<close>
+
+end
+
+subsection \<open> Further properties \<close>
+
+lemma (in wf_ast_problem) consts_objs_disj:
+  "fst ` set (consts D) \<inter> fst ` set (objects P) = {}"
+  using list.set_map wf_P(1) by auto
+
+lemma (in wf_ast_problem) objm_le_objT: "map_of (objects P) \<subseteq>\<^sub>m objT"
+proof -
+  have "dom constT \<inter> dom (map_of (objects P)) = {}"
+    using constT_def consts_objs_disj
+    by (simp add: dom_map_of_conv_image_fst)
+  thus ?thesis using objT_def
+    by (simp add: map_add_comm map_le_iff_map_add_commute)  
+qed
+
+lemma (in ast_domain) bigand_wf:
+  assumes "\<forall>\<phi> \<in> set \<phi>s. wf_fmla tyt \<phi>"
+  shows "wf_fmla tyt (\<^bold>\<And> \<phi>s)"
+  using assms by (induction \<phi>s; simp)
+
+lemma (in ast_domain) bigor_wf:
+  assumes "\<forall>\<phi> \<in> set \<phi>s. wf_fmla tyt \<phi>"
+  shows "wf_fmla tyt (\<^bold>\<Or> \<phi>s)"
+  using assms by (induction \<phi>s; simp)
+
+text \<open> Properties of sig \<close>
+
+abbreviation "split_pred \<equiv> (\<lambda>PredDecl p n \<Rightarrow> (p, n))"
+
+lemma split_pred_alt: "split_pred p = (pred p, argTs p)"
+  using predicate_decl.case_eq_if by auto
+
+lemma (in ast_domain) pred_resolve:
+  assumes "distinct (map pred (predicates D))"
+  shows "sig p = Some Ts \<longleftrightarrow> PredDecl p Ts \<in> set (predicates D)"
+proof -
+  let ?preds = "predicates D"
+  have "map (fst \<circ> split_pred) ?preds = map pred ?preds"
+    using split_pred_alt by simp
+  hence dis: "distinct (map (fst \<circ> split_pred) ?preds)"
+    using assms by metis
+
+  have "PredDecl p Ts \<in> set ?preds
+    \<longleftrightarrow> (p, Ts) \<in> set (map split_pred ?preds)"
+    using split_pred_alt by force
+  also have "... \<longleftrightarrow> map_of (map split_pred ?preds) p = Some Ts"
+    using dis by simp
+
+  ultimately show ?thesis using sig_def by simp
+qed
+
+lemmas (in wf_ast_domain) sig_Some = pred_resolve[OF wf_D(2)]
+
+lemma (in ast_domain) sig_None:
+    "sig p = None \<longleftrightarrow> p \<notin> pred ` set (predicates D)"
+  proof -
+    have "sig p = None \<longleftrightarrow> p \<notin> fst ` set (map split_pred (predicates D))"
+      using sig_def by (simp add: map_of_eq_None_iff)
+    also have "... \<longleftrightarrow> p \<notin> pred ` set (predicates D)"
+      using split_pred_alt by auto
+    ultimately show ?thesis by simp
+  qed
+
+text \<open> action parameters \<close>
+
+lemma (in ast_domain) ac_tsubst_intro:
+  assumes "distinct (map fst params)" "params ! i = (v, vT)" "args ! i = n" "i < length params" "i < length args"
+  shows "ac_tsubst params args (term.VAR v) = n"
+proof -
+  have "(v, n) \<in> set (zip (map fst params) args)"
+    using assms in_set_zip by fastforce
+  moreover have "distinct (map fst (zip (map fst params) args))"
+    using assms(1) by (simp add: map_fst_zip_take)
+  ultimately have "(the \<circ> map_of (zip (map fst params) args)) v = n"
+    by simp
+  thus ?thesis using ac_tsubst_def by fastforce
+qed
+
+text \<open> (Plan) Action instantiation \<close>
+
+(* only first condition matters in wf_ast_problem. See: res_aux*)
+lemma (in ast_problem) wf_pa_refs_ac:
+  assumes "wf_plan_action (PAction n args)"
+  obtains ac where "resolve_action_schema n = Some ac" "ac \<in> set (actions D)"
+    "ac_name ac = n" "action_params_match ac args"
+  using assms apply (cases "resolve_action_schema n")
+   apply simp
+  using resolve_action_schema_def index_by_eq_SomeD by fastforce
+
+lemma (in wf_ast_problem) res_aux:
+  "resolve_action_schema n = Some ac \<longleftrightarrow>
+     ac \<in> set (actions D) \<and> ac_name ac = n"
+  by (simp add: resolve_action_schema_def wf_D(6))
+
+theorem (in wf_ast_problem) wf_resolve_instantiate:
+  assumes "wf_plan_action \<pi>"
+  shows "wf_ground_action (resolve_instantiate \<pi>)"
+proof (cases \<pi>)
+  case [simp]: (PAction n args)
+  with assms obtain ac where
+    "resolve_action_schema n = Some ac" and
+    "action_params_match ac args" and
+    "ac \<in> set (actions D)"
+    using wf_pa_refs_ac by metis
+  thus ?thesis using wf_D(7) wf_instantiate_action_schema by simp
+qed
+
+theorem (in wf_ast_problem) wf_execute_stronger:
+    assumes "wf_plan_action \<pi>"
+    assumes "wf_world_model s"
+    shows "wf_world_model (execute_plan_action \<pi> s)"
+  proof (cases \<pi>)
+    case [simp]: (PAction name args)
+    from assms(1) have "wf_ground_action (resolve_instantiate \<pi>)"
+      using wf_resolve_instantiate by blast
+    thus ?thesis
+      apply (simp add: execute_plan_action_def execute_ground_action_def)
+      apply (rule wf_apply_effect)
+      apply (cases "resolve_instantiate \<pi>"; simp)
+      by (rule \<open>wf_world_model s\<close>)
+  qed
+
+text \<open> Semantics \<close>
+
+lemma entail_adds_irrelevant:
+  assumes "wm_basic M" "wm_basic A"
+          "A \<inter> Atom ` atoms \<F> = {}"
+  shows "M \<union> A \<^sup>c\<TTurnstile>\<^sub>= \<F> \<longleftrightarrow> M \<^sup>c\<TTurnstile>\<^sub>= \<F>"
+proof -
+  from assms(3) have "valuation (M \<union> A) \<Turnstile> \<F> \<longleftrightarrow> valuation M \<Turnstile> \<F>"
+  proof (induction \<F>)
+    case (Atom x)
+    thus ?case unfolding valuation_def by (cases x) simp_all
+  qed auto
+  moreover have "wm_basic (M \<union> A)" using assms(1-2) wm_basic_def by blast
+  ultimately show ?thesis using assms valuation_iff_close_world by metis
+qed
+
+lemma entail_dels_irrelevant:
+  assumes "wm_basic M" "wm_basic D"
+          "D \<inter> Atom ` atoms \<F> = {}"
+  shows "M - D \<^sup>c\<TTurnstile>\<^sub>= \<F> \<longleftrightarrow> M \<^sup>c\<TTurnstile>\<^sub>= \<F>"
+proof -
+  from assms(3) have "valuation (M - D) \<Turnstile> \<F> \<longleftrightarrow> valuation M \<Turnstile> \<F>"
+  proof (induction \<F>)
+    case (Atom x)
+    thus ?case unfolding valuation_def by (cases x) simp_all
+  qed auto
+  moreover have "wm_basic (M - D)" using assms(1-2) wm_basic_def by blast
+  ultimately show ?thesis using assms valuation_iff_close_world by metis
+qed
+
+end
